

## Course Format.

-  $\frac{1}{3}$  Lecture + -  $\frac{1}{3}$  Lab.

=

GLM. - Revisit to GLM. - from math./stat prospective.

### 1. Why GLM.

#### Linear Regression

Assume.  $Y_1, \dots, Y_n$  ind., satisfy  $E(Y_i) = x_i^T \beta$ .

$x_i$  - observed predictors / covariates.

$\beta$  - regression coefficients.

→ If we further assume

$$Y_i \stackrel{\text{ind}}{\sim} N(x_i^T \beta, \sigma^2), \quad i=1, \dots, n \quad \sigma^2 > 0, \text{ unknown.}$$

ordinary linear regression.

exact inference about  $\beta$ . based on t, & F tests.

→ If we drop normality assumption.

$$Y_i \stackrel{\text{ind}}{\sim} (x_i^T \beta, \sigma^2), \quad i=1, \dots, n.$$

when  $n$  is large.

robust. to violation  
standard tests. CI. are approximately correct.

\* In many situations even these weakened assumption are untenable.

•  $\mu(x) := E(Y|x)$  is not a linear function of  $x$

•  $\text{Var}(Y_i)$  is not constant in  $i$

#### Possible solution

- weighted least squares. if  $\text{Var}(Y_i) = a_i^2 \sigma^2$ .  $a_1, \dots, a_n$  are known constants

- transformation of  $\vec{x}$  to correct nonlinearity. ← Focus. [Figure 8.3. CASI].

- transformation of  $Y$  if either  $\mu(x) = E(Y|x)$  is nonlinear.

or  $\sigma^2(x) := \text{Var}(Y|x)$  is not constant in  $\vec{x}$

## 2. Defining GLM.

Systematic Component.  $\xrightarrow{\text{relates}} \text{predictors } \bar{X} = (x_1, \dots, x_p).$   
to the mean response  $\mu = E(Y).$

• the linear predictor:  $\eta = \bar{X}^T \bar{\beta}$

• the link function:  $g(\mu) = \eta$ , where  $g$  is a smooth, monotonic function.

Example.

- Gaussian identity.
- binary. logit.

Random (Stochastic) Component  $\xrightarrow{\text{specifies}} \text{distributional form of the responses.}$  It assume

•  $Y_1, \dots, Y_n$  ind.

•  $Y_i$  has density  $f(\cdot; \theta_i, \phi_i)$ ,  $\phi_i = \phi/a_i$ ,  $\phi > 0$ . where  $a_1, \dots, a_n$  are known.  
and  $f$  has the form

$$f(y; \theta, \phi) = \exp \left\{ \frac{y\theta - b(\theta)}{\phi} + c(y; \phi) \right\}.$$

$\rightarrow$  dispersion parameter.

For fixed  $\phi$ ,  $f(\cdot; \theta, \phi)$  defines a one-parameter exponential family.  
 $\uparrow$   
canonical parameter.

Let  $l(\theta, \phi) = \log f(y; \theta, \phi) = \frac{1}{\phi} [y\theta - b(\theta)] + c(y; \phi).$

HW?

Then  $\frac{\partial l}{\partial \theta} = \frac{1}{\phi} [y - b'(\theta)].$

From the first two Bartlett identities

$$E_{\theta, \phi} \left( \frac{\partial l}{\partial \theta} \right) = 0, \quad E_{\theta, \phi} \left[ \left( \frac{\partial l}{\partial \theta} \right)^2 \right] = E_{\theta, \phi} \left( - \frac{\partial^2 l}{\partial \theta^2} \right).$$

$$\frac{\partial^2 l}{\partial \theta^2} = - \frac{1}{\phi} b''(\theta).$$

$$\Rightarrow E_{\theta, \phi}(Y) = b'(\theta), \quad \text{Var}_{\theta, \phi}(Y) = \phi b''(\theta). \quad \begin{array}{l} \text{Var}(Y) > 0 \\ \phi > 0 \end{array} \quad \begin{array}{l} b''(\theta) > 0. \\ \downarrow \\ b'(\theta) \uparrow. \end{array}$$

$$\Rightarrow \theta = (b')^{-1}(\mu).$$

$$\mu = g^{-1}(\eta) = g^{-1}(\bar{X}^T \bar{\beta}).$$

$$\Rightarrow \theta = (b')^{-1}(g^{-1}(\bar{X}^T \bar{\beta})).$$

• The function  $(b')^{-1}(\mu)$  — canonical link.

If we choose  $g = (b')^{-1}$

$$\theta = \bar{X}^T \bar{\beta} = \eta. \quad - \text{simplifies calculations.}$$

$$g'(\mu) = \frac{1}{b''((b')^{-1}(\mu))} = \frac{1}{V(\mu)}$$

Give an.

Example. poisson ( $\mu$ ). [Example 1.7] variance function.

HW on. Binomial.  $\rightarrow$  logistic.

### 3 The GLM Likelihood.

Recall that in a GLM,  $Y_1, \dots, Y_n$  are independent with.

$$Y_i \sim f(\cdot; \theta_i, \phi_i), \quad \phi_i = \phi / a_i. \quad \text{where.}$$

$$f(y; \theta, \phi) = \exp \left\{ \frac{y\theta - b(\theta)}{\phi} + c(y; \phi) \right\}.$$

Further.  $\theta_i$  is a function of  $\mu_i$ :  $\mu_i = b'(\theta_i) \Rightarrow \theta_i = (b')^{-1}(\mu_i)$ ;

$\mu_i$  is a function of  $\eta_i$ :  $g(\mu_i) = \eta_i \Rightarrow \mu_i = g^{-1}(\eta_i)$ ;

$\eta_i$  is a function of  $\beta$ :  $\eta_i = \vec{x}_i^T \vec{\beta}$

$\Rightarrow$  each  $\theta_i$  is a function of the unknown  $\vec{\beta}$ , while  $\phi$  (known or unknown) is free of  $\vec{\beta}$ .

$\hookrightarrow$  Need to estimate  $\vec{\beta}$  and possibly  $\phi$ .

#### - Likelihood Equations for the Regression Coefficients

The contribution of the  $i$ -th observation to the log-likelihood is.

$$l_i(\vec{\beta}, \theta) = \log f(y_i; \theta_i, \phi/a_i) = \frac{y_i \theta_i - b(\theta_i)}{\phi/a_i} + c(y_i; \phi/a_i)$$

$$\Rightarrow l = \sum_{i=1}^n l_i, \quad \phi \text{ does not depend on } \vec{\beta}$$

$$\text{By the chain rule, } \frac{\partial l_i}{\partial \beta_j} = \frac{\partial l_i}{\partial \theta_i} \cdot \frac{\partial \theta_i}{\partial \beta_j} + \underbrace{\frac{\partial l_i}{\partial \phi} \cdot \frac{\partial \phi}{\partial \beta_j}}_{=0} = \frac{\partial l_i}{\partial \theta_i} \cdot \frac{\partial \theta_i}{\partial \mu_i} \cdot \frac{\partial \mu_i}{\partial \eta_i} \cdot \frac{\partial \eta_i}{\partial \beta_j}$$

Let  $V(\mu) = b''((b')^{-1}(\mu))$  be the variance function.  $\Rightarrow \text{Var}(Y) = \phi V(\mu)$ .

$$\text{Then } \frac{\partial l_i}{\partial \theta_i} = \frac{1}{\phi} a_i (y_i - \mu_i) \quad \mu_i = b'(\theta_i)$$

$$\frac{\partial \theta_i}{\partial \mu_i} = \frac{1}{\partial \mu_i / \partial \theta_i} = \frac{1}{b''(\theta_i)} = \frac{1}{b''((b')^{-1}(\mu_i))} = \frac{1}{V(\mu_i)}$$

$$\frac{\partial \mu_i}{\partial \eta_i} = \frac{1}{\partial \eta_i / \partial \mu_i} = \frac{1}{g'(\mu_i)}$$

$$\Rightarrow \frac{\partial l_i}{\partial \beta_j} = \frac{1}{\phi} \frac{a_i (y_i - \mu_i)}{V(\mu_i) g'(\mu_i)} \cdot x_{ij}$$

$$\eta_i = \vec{x}_i^T \vec{\beta} = \sum_{j=1}^p x_{ij} \beta_j$$

$$\frac{\partial \eta_i}{\partial \beta_j} = x_{ij}$$

$$\Rightarrow \frac{\partial l}{\partial \beta_j} = \sum_{i=1}^n \frac{\partial l_i}{\partial \beta_j} = \frac{1}{\phi} \sum_{i=1}^n \frac{a_i (y_i - \mu_i)}{V(\mu_i) g'(\mu_i)} x_{ij}$$

MLE of  $\vec{\beta}$ .  $\frac{\partial L}{\partial \beta_j} = 0$ .

Likelihood equation for  $\vec{\beta}$

$$\Rightarrow \sum_{i=1}^n \frac{a_i (y_i - \mu_i)}{v(\mu_i) g'(\mu_i)} x_{ij} = 0 \quad j = 1, \dots, p. \quad \text{for } \vec{\beta} = (\beta_1, \dots, \beta_p)^T.$$

- Fisher Information.

[ Definition ] - quantifies how much information an observed r.v.  $X$  carries about an unknown parameter  $\theta$  of a statistical model.

Formally, for a likelihood  $L(\theta; X)$

$$I(\theta) = E \left[ \left( \frac{\partial}{\partial \theta} \log L(\theta; X) \right)^2 \right].$$

Assume  $\phi$  is known. the observed Fisher Information is  $I(\hat{\beta})$ .  $\hat{\beta}$  is the MLE of  $\vec{\beta}$ .

$$I(\beta) = - \frac{\partial^2 L}{\partial \vec{\beta} \partial \vec{\beta}^T} = \left( - \frac{\partial^2 L}{\partial \beta_j \partial \beta_k} \right)_{1 \leq j, k \leq p} \quad - \text{negative - Hessian of the log-likelihood.}$$

Note  $\frac{\partial^2 L_i}{\partial \beta_j \partial \beta_k} = \frac{\partial}{\partial \beta_k} \left( \frac{1}{\phi} \frac{a_i (y_i - \mu_i)}{v(\mu_i) g'(\mu_i)} x_{ij} \right) = \frac{\partial}{\partial \mu_i} \left( \frac{1}{\phi} \frac{a_i (y_i - \mu_i)}{v(\mu_i) g'(\mu_i)} x_{ij} \right) \cdot \frac{\partial \mu_i}{\partial \beta_k}$

$$\frac{\partial}{\partial \mu_i} \left( \frac{1}{\phi} \frac{a_i (y_i - \mu_i)}{v(\mu_i) g'(\mu_i)} x_{ij} \right) = - \frac{1}{\phi} \frac{a_i}{v(\mu_i) g'(\mu_i)} x_{ij} + \frac{1}{\phi} a_i (y_i - \mu_i) \cdot \frac{\partial}{\partial \mu_i} \left( \frac{1}{v(\mu_i) g'(\mu_i)} \right)$$

$$\frac{\partial \mu_i}{\partial \beta_k} = \frac{\partial \mu_i}{\partial \eta_i} \cdot \frac{\partial \eta_i}{\partial \beta_k} = \frac{1}{g'(\mu_i)} x_{ik}.$$

$$\Rightarrow I(\beta)_{j,k} = - \sum_{i=1}^n \frac{\partial^2 L_i}{\partial \beta_j \partial \beta_k} = \frac{1}{\phi} \sum_{i=1}^n \left\{ \frac{a_i}{v(\mu_i) g'(\mu_i)^2} - \frac{a_i (y_i - \mu_i)}{g'(\mu_i)} \frac{\partial}{\partial \mu_i} \left( \frac{1}{v(\mu_i) g'(\mu_i)} \right) \right\} x_{ij} x_{ik}.$$

↓  
depend on  $\vec{\beta}$  through  $\mu_i$

$$\Rightarrow I(\vec{\beta}) = E_{\vec{\beta}} [ I(\vec{\beta}) ]. \quad \text{since only } y_i \text{ are random. } \& \quad E[(Y_i - \mu_i)] = 0.$$

$$I(\beta)_{j,k} = \frac{1}{\phi} \sum_{i=1}^n \frac{a_i}{v(\mu_i) g'(\mu_i)^2} x_{ij} x_{ik}.$$

Let  $W = W(\vec{\beta}) = \text{diag} \left\{ \frac{a_i}{v(\mu_i) g'(\mu_i)^2} : i = 1, \dots, n \right\}.$

$$\Rightarrow I(\vec{\beta}) = \frac{1}{\phi} X^T W X.$$

? HW. canonical case.

Large sample theory. MLE of  $\vec{\beta}$ .  $\hat{\vec{\beta}} \sim AN(\vec{\beta}, \phi (X^T W X)^{-1})$  as  $n \rightarrow \infty$ .



#### 4. Computation of Estimators.

— Newton's method.

— Iteratively reweighted least squares.

#### 5. Deviance - a measure of fit.

analogous the ~~sum~~ residual sum of squares in Linear regression.

$$\text{Let } l(\mu, \phi; y) = \sum_{i=1}^n \log f(y_i; \theta_i, \phi/a_i) = \frac{1}{\phi} \sum_{i=1}^n a_i [y_i \theta_i - b(\theta_i)] + \sum_{i=1}^n c(y_i; \phi/a_i)$$

where  $\theta_i = (b')^{-1}(\mu_i)$ .

For GLM with  $\eta_i = x_i^T \beta$  &  $g(\mu_i) = \eta_i$ ,  $i=1, \dots, n$

let  $\hat{\beta}$  be the MLE, and let.

$$\hat{\eta}_i = x_i^T \hat{\beta}, \quad \hat{\mu}_i = g^{-1}(\hat{\eta}_i), \quad \hat{\theta}_i = (b')^{-1}(\hat{\mu}_i), \quad \text{and} \quad \tilde{\theta}_i = (b')^{-1}(y_i).$$

Def. With the notation above, the deviance for the fitted GLM model is

$$D(\bar{y}; \hat{\mu}) = 2 [l(\bar{y}, \phi; \bar{y}) - l(\hat{\mu}, \phi; \bar{y})] \cdot \phi$$

$$= \sum_{i=1}^n 2 a_i \{ y_i (\tilde{\theta}_i - \hat{\theta}_i) - [b(\tilde{\theta}_i) - b(\hat{\theta}_i)] \}. \quad \rightarrow \text{Does not depend on } \phi$$

and the scaled deviance is

$$D^*(\bar{y}; \hat{\mu}) = \frac{1}{\phi} D(\bar{y}; \hat{\mu}).$$



It is twice the "Kullback-Leibler" distance

\* GLM. Maximum likelihood fitting is "least total deviance" in the same way that linear regression is least sum of squares.

i.e. the MLE  $\hat{\beta}$  is the choice of  $\beta$  that minimizes the total deviance.

#### — Analysis of Deviance.

Suppose  $M_0 < M_1$ .  $\hat{\beta}_0, \hat{\beta}_1$  corresponding MLE with  $\hat{\mu}_0, \hat{\mu}_1$ . Assume  $\phi$  is known.

the likelihood ratio test statistics for  $H_0: M_0$  is the true model

vs  $H_1: M_1$  is the true model.

$$T_{LR} = -2 [l(\hat{\mu}_0, \phi; \bar{y}) - l(\hat{\mu}_1, \phi; \bar{y})] = \frac{1}{\phi} [D(\bar{y}; \hat{\mu}_0) - D(\bar{y}; \hat{\mu}_1)] = D^*(\bar{y}, \hat{\mu}_0) - D^*(\bar{y}, \hat{\mu}_1)$$

$$\xrightarrow[\text{Ho}]{d} \chi_r^2 \quad \text{as } n \rightarrow \infty.$$

$r$ : difference in the # of para. between  $M_0$  &  $M_1$ .

We reject  $M_0$  if  $T_{LR} > \chi_{r, \alpha}^2$ .